\begin{table}[t]
%\begin{table*}[t]
\centering
\input{decrement-logic/tables/table8.tex}
\begin{align}
    A &= W_1' \\
    B &= (X_1' W_1' ((Z_1' Y_1) + (Z_1 Y_1'))) + (Z_1' W_1 X_1) \\
    C &= (Z_1' Y_1 (X_1 + W_1)) + (Z_1 X_1' W_1' Y_1') \\
    D &= X_1' Y_1' ((Z_1 W_1) + (Z_1' W_1')) 
\end{align}
\input{decrement-logic/tables/table9.tex}
\begin{align}
    A &= W_2' \\
    B &= (Y_2 X_2' W_2') + (Y_2' X_2 W_2) \\
    C &= X_2' ((Y_2 W_2) + (Y_2' W_2')) \\
    D &= 0 
\end{align}
\input{decrement-logic/tables/table10.tex}
\begin{align}
    A &= W_5' \\
    B &= (X_5 W_5) + (X_5' W_5') \\
    C &=D= 0 
\end{align}
\input{decrement-logic/tables/table11.tex}
\begin{align}
    A &= X_6 W_6' \\
    B &= X_6' W_6' \\
    C &=D= 0 
\end{align}
\caption{Truth Tables for decrementing displays}
\label{tab:decrement}
%\end{table}
\end{table}
